LL1/Proofs/Parser/SoundnessNoFuel.v
@@ -13,25 +13,30 @@ Import ListNotations.
 
 Lemma parse_nf_eq_body :
   forall tbl sym input vis a,
-    parse_nf tbl sym input vis a = 
-  match (sym, input) with
-  | (T _, nil) => inl (Reject "input exhausted" input)
-  | (T y, token :: input') =>
-    if string_dec y token then
-      inr (Leaf y, input')
-    else
-      inl (Reject "token mismatch" input)
-  | (NT x, _) =>
+    parse_nf tbl sym input vis a =
+      match sym with
+  | T a =>
+    match input as i return input = i -> _ with
+    | nil =>
+      fun _ => inl (Reject "input exhausted" input)
+    | token :: input' => 
+      fun Hin => 
+        if string_dec a token then
+          inr (Leaf a, existT _ input' (length_lt_eq_cons _ _ _ _ Hin))
+        else
+          inl (Reject "token mismatch" input)
+    end eq_refl
+  | NT x =>
     match ptlk_dec x (peek input) tbl with
     | inl _ => inl (Reject "lookup failure" input)
     | inr (exist _ gamma Hlk) =>
       match mem_dec x vis with
       | left _ => inl (LeftRec x vis input)
-      | right Hnin => 
-        match parseForest_nf tbl gamma input (NtSet.add x vis) (hole1 _ _ _ _  _ _ _ a Hlk Hnin) with
+      | right Hnin =>
+        match parseForest_nf tbl gamma input (NtSet.add x vis) (hole1 _ _ _ _ _ _ _ a Hlk Hnin) with
         | inl pfail => inl pfail
-        | inr (sts, input') =>
-          inr (Node x sts, input')
+        | inr (sts, existT _ input' Hle) =>
+          inr (Node x sts, existT _ input' Hle)
         end
       end
     end
@@ -43,24 +48,25 @@ Qed.
 Lemma parseForest_nf_eq_body :
   forall tbl gamma input vis a,
     parseForest_nf tbl gamma input vis a =
-    match gamma as g return gamma = g -> _  with
-    | nil => fun _ => inr (nil, input)
+        match gamma as g return gamma = g -> _  with
+    | nil => fun _ => inr (nil, existT (fun input' => length_lt_eq string input' input) input
+                                       (length_lt_eq_refl _ _))
     | sym :: gamma' => fun Hg => 
                          match parse_nf tbl sym input vis (hole2 _ _ _ _ _ a) with
                          | inl pfail => inl pfail
-                         | inr (lSib, input') =>
-                           match Compare_dec.lt_dec (List.length input') (List.length input) with
+                         | inr (lSib, existT _ input' Hle) =>
+                           match Hle with
                            | left Hlt =>
                              match parseForest_nf tbl gamma' input' NtSet.empty (hole3 _ _ _ _ _ _ _ a Hlt) with
                              | inl pfail => inl pfail
-                             | inr (rSibs, input'') =>
-                               inr (lSib :: rSibs, input'')
+                             | inr (rSibs, existT _ input'' Hle'') =>
+                               inr (lSib :: rSibs, existT _ input'' (length_lt_eq_trans _ _ _ _ Hle'' Hle))
                              end
-                           | right Hnlt =>
+                           | right Heq =>
                              match parseForest_nf tbl gamma' input vis (hole4 _ _ _ _ _ _ a Hg) with
                              | inl pfail => inl pfail
-                             | inr (rSibs, input'') =>
-                               inr (lSib :: rSibs, input'')
+                             | inr (rSibs, existT _ input'' Hle'') =>
+                               inr (lSib :: rSibs, existT _ input'' Hle'')
                              end
                            end
                          end
@@ -97,6 +103,15 @@ Proof.
   inv H; auto.
 Qed.
 
+Lemma lengths_contra :
+  forall A (xs ys : list A),
+    List.length xs = List.length ys
+    -> List.length xs < List.length ys
+    -> False.
+Proof.
+  intros; omega.
+Qed.
+
 Lemma input_length_invariant :
   forall (g   : grammar)
          (tbl : parse_table),
@@ -104,11 +119,12 @@ Lemma input_length_invariant :
     -> forall (tr        : tree)
               (sym       : symbol)
               (input rem : list terminal)
+              Hle
               (vis       : NtSet.t)
               (a : Acc triple_lt (meas tbl input vis (F_arg sym))),
-      parse_nf tbl sym input vis a = inr (tr, rem)
+      parse_nf tbl sym input vis a = inr (tr, existT _ rem Hle)
       -> List.length rem < List.length input
-         \/ (nullable_sym g sym /\ rem = input).
+         \/ nullable_sym g sym.
 Proof.
   intros g tbl Htbl tr.
   induction tr as [ s
@@ -120,11 +136,12 @@ Proof.
       (Q := fun f =>
               forall (gamma : list symbol)
                      (input rem : list string)
+                     Hle
                      (vis : NtSet.t)
                      (a   : Acc triple_lt (meas tbl input vis (G_arg gamma))),
-                parseForest_nf tbl gamma input vis a = inr (f, rem)
+                parseForest_nf tbl gamma input vis a = inr (f, existT _ rem Hle)
                 -> List.length rem < List.length input
-                   \/ (nullable_gamma g gamma /\ rem = input)); intros; destruct a.
+                   \/ nullable_gamma g gamma); intros; destruct a.
 
   - destruct sym as [y | x].
     + cr; tc.
@@ -138,39 +155,36 @@ Proof.
       step; tc.
       step_eq Hpf; tc.
       step.
+      step.
       inv H.
-      apply IHpf in Hpf.
+      apply IHpf in Hpf; clear IHpf.
       destruct Hpf; auto.
-      destruct H; subst.
-      right; split; auto.
+      right.
       apply Htbl in e; destruct e.
       econstructor; eauto.
 
   - cr; tc.
-    inv H; auto.
 
   - step; tc.
     step_eq Hp; tc.
     step.
     step.
-    + step_eq Hpf; tc.
+    step.
+    + left.
+      step_eq Hpf; tc.
+      step.
+      step.
+      inv H.
+      destruct l1; subst; omega.
+    + subst.
+      step_eq Hpf; tc.
+      step.
       step.
       inv H.
       apply IHp in Hp; clear IHp.
       apply IHpf in Hpf; clear IHpf.
-      destruct Hpf.
-      * left; omega.
-      * destruct H; subst; auto. 
-    + step_eq Hpf; tc.
-      step.
-      inv H.
-      apply IHp in Hp; clear IHp.
-      destruct Hp.
-      * contradiction.
-      * destruct H; subst.
-        apply IHpf in Hpf; clear IHpf.
-        destruct Hpf; auto.
-        destruct H0; subst; auto.
+      destruct Hp; try omega.
+      destruct Hpf; auto.
 Qed.
 
 Lemma parse_sound' :
@@ -180,9 +194,10 @@ Lemma parse_sound' :
     -> forall (tr        : tree)
               (sym       : symbol)
               (input rem : list terminal)
+              Hle
               (vis       : NtSet.t)
               (a : Acc triple_lt (meas tbl input vis (F_arg sym))),
-      parse_nf tbl sym input vis a = inr (tr, rem)
+      parse_nf tbl sym input vis a = inr (tr, existT _ rem Hle)
       -> exists word,
         word ++ rem = input
         /\ (@sym_derives_prefix g) sym word tr rem.
@@ -197,9 +212,10 @@ Proof.
       (Q := fun f =>
               forall (gamma : list symbol)
                      (input rem : list string)
+                     Hle
                      (vis : NtSet.t)
                      (a   : Acc triple_lt (meas tbl input vis (G_arg gamma))),
-                parseForest_nf tbl gamma input vis a = inr (f, rem)
+                parseForest_nf tbl gamma input vis a = inr (f, existT _ rem Hle)
                 -> exists word,
                   word ++ rem = input
                   /\ gamma_derives_prefix gamma word f rem); intros; destruct a.
@@ -222,6 +238,7 @@ Proof.
       step; tc.
       step_eq Hpf; tc.
       step.
+      step.
       inv H.
       apply IHpf in Hpf; clear IHpf.
       destruct Hpf as [word [Happ Hg]]; subst.
@@ -240,7 +257,10 @@ Proof.
     step_eq Hp; tc.
     step.
     step.
-    + step_eq Hpf; tc.
+    step.
+    + (* length_lt case *)
+      step_eq Hpf; tc.
+      step; tc.
       step.
       inv H.
       apply IHp in Hp; clear IHp.
@@ -250,15 +270,13 @@ Proof.
       exists (wpre ++ wsuf); split.
       * rewrite app_assoc; auto.
       * constructor; auto.
-    + pose proof Hp as Hp'.
-      eapply input_length_invariant in Hp'; eauto.
-      destruct Hp'; try contradiction.
-      destruct H0; subst.
+    + subst.
       step_eq Hpf; tc.
       step.
+      step.
       inv H.
-      apply IHp in Hp; clear IHp.
-      apply IHpf in Hpf; clear IHpf.
+      eapply IHp in Hp; clear IHp.
+      eapply IHpf in Hpf; clear IHpf.
       destruct Hp as [wpre [Happ Hs]].
       apply l_ident_eq_nil in Happ; subst.
       destruct Hpf as [wsuf [Happ Hg]]; subst.
@@ -273,12 +291,13 @@ Lemma parse_sound :
     -> forall (tr        : tree)
               (sym       : symbol)
               (word rem  : list terminal)
+              Hle
               (vis       : NtSet.t)
               (a : Acc triple_lt (meas tbl (word ++ rem) vis (F_arg sym))),
-      parse_nf tbl sym (word ++ rem) vis a = inr (tr, rem)
+      parse_nf tbl sym (word ++ rem) vis a = inr (tr, existT _ rem Hle)
       -> (@sym_derives_prefix g) sym word tr rem.
 Proof.
-  intros g tbl Htbl tr sym word rem vis a Hp.
+  intros g tbl Htbl tr sym word rem Hle vis a Hp.
   pose proof Hp as Hp'.
   eapply parse_sound' in Hp; eauto.
   destruct Hp as [word' [Happ Hder]].
